testdata/cue/unresolved_builtin.expected
@@ -1,0 +1,2 @@
+lenString: len(string)
+emptyOr: or([])
